Logic/Modal/Normal/Formula.lean
@@ -208,94 +208,33 @@ namespace Theory
 
 variable (Γ : Theory α)
 
-def box : Theory α := .box '' Γ
+@[simp] abbrev box : Theory α := Set.box Γ
 prefix:74 "□" => Theory.box
 
-@[simp]
-lemma box_empty : □(∅ : Theory α) = ∅ := by simp [box]
-
-@[simp]
-lemma box_subset {Γ Δ : Theory α} (d : Γ ⊆ Δ) : □Γ ⊆ □Δ := by
-  simp_all [box, Set.subset_def];
-
-lemma box_union {Γ Δ : Theory α} : □(Γ ∪ Δ) = □Γ ∪ □Δ := by
-  simp_all [box, Set.image_union]
-
-lemma box_mem {Γ : Theory α} : p ∈ □Γ ↔ (∃ q ∈ Γ, □q = p) := by
-  simp_all [box]
-  rfl;
-
-def dia : Theory α := .dia '' Γ
+@[simp] abbrev dia : Theory α := Set.dia Γ
 prefix:74 "◇" => Theory.dia
-
-@[simp]
-lemma dia_empty : ◇(∅ : Theory α) = ∅ := by simp [dia]
-
-@[simp]
-lemma dia_subset {Γ Δ : Theory α} (d : Γ ⊆ Δ) : ◇Γ ⊆ ◇Δ := by
-  simp_all [dia, Set.subset_def];
-
-lemma dia_union {Γ Δ : Theory α} : ◇(Γ ∪ Δ) = ◇Γ ∪ ◇Δ := by
-  simp_all [dia, Set.image_union]
-
-lemma dia_mem {Γ : Theory α} : p ∈ ◇Γ ↔ (∃ q ∈ Γ, ◇q = p) := by
-  simp_all [dia]
-  rfl;
 
 def prebox : Theory α := .box ⁻¹' Γ
 prefix:73 "□⁻¹" => Theory.prebox
 
-def box_prebox {Γ} : □(□⁻¹Γ) = { □p | (p : Formula α) (_ : □p ∈ Γ) } := by aesop;
-
-@[simp]
-def box_prebox_subset {Γ : Theory α} : □(□⁻¹Γ) ⊆ Γ := by simp [box_prebox, Set.subset_def];
-
-@[simp]
-lemma prebox_subset {Γ Δ : Theory α} (d : Γ ⊆ Δ) : □⁻¹Γ ⊆ □⁻¹Δ := by
-  simp_all [prebox, Set.subset_def];
-
 def predia : Theory α := .dia ⁻¹' Γ
 prefix:73 "◇⁻¹" => Theory.predia
 
-@[simp]
-lemma predia_subset {Γ Δ : Theory α} (d : Γ ⊆ Δ) : ◇⁻¹Γ ⊆ ◇⁻¹Δ := by
-  simp_all [predia, Set.subset_def];
-
-def dia_predia {Γ} : ◇(◇⁻¹Γ) = { ◇p | (p : Formula α) (_ : ◇p ∈ Γ) } := by aesop;
-
-@[simp]
-def dia_predia_subset {Γ : Theory α} : ◇(◇⁻¹Γ) ⊆ Γ := by simp [dia_predia, Set.subset_def];
-
 end Theory
+
 
 abbrev Context (α : Type u) := Finset (Formula α)
 
 namespace Context
 
--- instance : Coe (Context α) (Theory α) := ⟨Finset.toSet⟩
-
 variable [DecidableEq α]
 variable (Γ : Context α)
 
-def box : Context α := Γ.image Formula.box
+abbrev box : Context α := Finset.box Γ
 prefix:73 "□" => box
 
-lemma box_union {Γ₁ Γ₂ : Context α} : (□(Γ₁ ∪ Γ₂) : Context α) = (□Γ₁ ∪ □Γ₂ : Context α) := by
-  simp only [Theory.box, Context.box, Finset.image_union]
-
-@[simp]
-lemma box_coe : (□(↑Γ : Theory α)) = ↑(□Γ : Context α) := by
-  simp only [Theory.box, Context.box, Finset.coe_image];
-
-def dia : Context α := Γ.image Formula.dia
+def dia : Context α := Finset.dia Γ
 prefix:73 "◇" => dia
-
-lemma dia_union {Γ₁ Γ₂ : Context α} : (◇(Γ₁ ∪ Γ₂) : Context α) = (◇Γ₁ ∪ ◇Γ₂ : Context α) := by
-  simp only [Theory.dia, Context.dia, Finset.image_union]
-
-@[simp]
-lemma dia_coe : (◇(↑Γ : Theory α)) = ↑(◇Γ : Context α) := by
-  simp only [Theory.dia, Context.dia, Finset.coe_image];
 
 end Context
 
